semantics: improve proof tools, but not the proofs nor UB
* Change the proof style from "unfolding" to "rewriting", with a number
  of built-in simp lemmas for Fitree. However, did NOT change the
  proofs in ArithSemantics.lean because they break constantly.
* Properly classify interpretation functions, now consistently named
  `interpMonad` for the interpreter `Fitree E ~> MonadT M`, and used in
  every relevant location.
* Did NOT update UB yet as it contributed a lot to the breakage.

Note:
* `simp_itree` is very fragile and often breaks for syntactic reasons.
  Ideally we'd deprecate it soon, but it's still the only way to get
  the proofs in ArithSemantics.lean to go through.

MLIR/Examples/SemanticsTests.lean
@@ -18,9 +18,9 @@ def Test.run (t: Test): String :=
   let (@Test.mk α σ ε δ S _ r) := t
   let t := semanticsRegion 99 r []
   let t := interp_ub! t
-  let t := interp_ssa t SSAEnv.empty
-  let t := interp' S.handle t
-  let t := interp ControlFlowOp.handleLogged t
+  let t := interpSSA' t SSAEnv.empty
+  let t := t.interp' S.handle
+  let t := t.interp ControlFlowOp.handleLogged
   t.run.run.snd
 
 def trueval := Test.mk (func_ + arith) "trueval.mlir" [mlir_region| {
