MLIR/Semantics/Fitree.lean
@@ -49,16 +49,17 @@ infixr:60 " +' " => sum1
 class Member (E: Type → Type) (F: Type → Type) where
   inject : E ~> F
 
-instance {E}: Member E E where
+instance MemberId {E}: Member E E where
   inject := (fun _ => id)
 
-instance {E F G} [Member E F]: Member E (F +' G) where
+instance MemberSumL {E F G} [Member E F]: Member E (F +' G) where
   inject T := Sum.inl ∘ Member.inject T
 
-instance {E F G} [Member E G]: Member E (F +' G) where
+instance MemberSumR {E F G} [Member E G]: Member E (F +' G) where
   inject T := Sum.inr ∘ Member.inject T
 
-instance {E F G H} [Member E G] [Member F H]: Member (E +' F) (G +' H) where
+instance MemberSum {E F G H} [Member E G] [Member F H]:
+    Member (E +' F) (G +' H) where
   inject T := Sum.cases (Member.inject T) (Member.inject T)
 
 -- Effects can now be put in context automatically by typeclass resolution
@@ -67,22 +68,6 @@ example E F:    Member E (E +' F) := inferInstance
 example E F:    Member E (F +' (F +' E)) := inferInstance
 example E F G:  Member (E +' F) (E +' F +' G) := inferInstance
 
-@[simp_itree]
-def Fitree.case_ (h1: E ~> G) (h2: F ~> G): E +' F ~> G :=
-  fun R ef => match ef with
-  | Sum.inl e => h1 R e
-  | Sum.inr f => h2 R f
-
-
-/- Examples of interactions -/
-
-inductive StateE {S: Type}: Type → Type where
-  | Read: Unit → StateE S
-  | Write: S → StateE PUnit
-
-inductive WriteE {W: Type}: Type → Type where
-  | Tell: W → WriteE Unit
-
 
 /- The monadic domain; essentially finite Interaction Trees -/
 
@@ -90,7 +75,6 @@ inductive Fitree (E: Type → Type) (R: Type) where
   | Ret (r: R): Fitree E R
   | Vis {T: Type} (e: E T) (k: T → Fitree E R): Fitree E R
 
-@[simp_itree]
 def Fitree.ret {E R}: R → Fitree E R :=
   Fitree.Ret
 
@@ -110,52 +94,6 @@ instance {E}: Monad (Fitree E) where
   pure := Fitree.ret
   bind := Fitree.bind
 
-
-@[simp_itree]
-def Fitree.translate {E F R} (f: E ~> F): Fitree E R → Fitree F R
-  | Ret r => Ret r
-  | Vis e k => Vis (f _ e) (fun r => translate f (k r))
-
--- TODO: consider making this a coercion
-def Fitree.inject {E: Type → Type} {F: Type → Type} {T} [Member E F]
-    (fe: Fitree E T): Fitree F T := Fitree.translate Member.inject fe
-
--- Interpretation into the monad of finite ITrees
-@[simp_itree]
-def interp {M} [Monad M] {E} (h: E ~> M):
-    forall {R}, Fitree E R → M R :=
-  fun t =>
-    match t with
-    | Fitree.Ret r => pure r
-    | Fitree.Vis e k => bind (h _ e) (fun t => interp h (k t))
-
-@[simp_itree]
-def interp' {E F} (h: E ~> Fitree Void1):
-    forall {R}, Fitree (E +' F) R → Fitree F R :=
-  fun t =>
-    interp (Fitree.case_
-      (fun _ e => (h _ e).translate $ fun _ e => nomatch e)
-      (fun _ e => Fitree.trigger e)) t
-
--- Interpretation into the state monad. This is semantically equivalent to
--- `interp`, but the specialization is useful to write state-specific theorems.
-@[simp_itree]
-def interp_state {M S} [Monad M] {E} (h: E ~> StateT S M):
-    forall {R}, Fitree E R → StateT S M R :=
-  interp h
-
--- Interpretation into the writer monad
-@[simp_itree]
-def interp_writer {M} [Monad M] {E} (h: E ~> WriterT M):
-    forall {R}, Fitree E R → WriterT M R :=
-  interp h
-
--- Interpretation into the option monad
-@[simp_itree]
-def interp_option {M} [Monad M] {E} (h: E ~> OptionT M):
-    forall {R}, Fitree E R → OptionT M R :=
-  interp h
-
 -- Since we only use finite ITrees, we can actually run them when they're
 -- fully interpreted (which leaves only the Ret constructor)
 @[simp_itree]
@@ -163,17 +101,335 @@ def Fitree.run {R}: Fitree Void1 R → R
   | Ret r => r
   | Vis e _ => nomatch e
 
+@[simp] theorem Fitree.run_ret:
+  Fitree.run (Fitree.ret r) = r := rfl
 
-/- Predicates to reason about the absence of events -/
+@[simp_itree]
+def Fitree.translate {E F R} (f: E ~> F): Fitree E R → Fitree F R
+  | Ret r => Ret r
+  | Vis e k => Vis (f _ e) (fun r => translate f (k r))
 
-inductive Fitree.no_event_l {E F R}: Fitree (E +' F) R → Prop :=
-  | Ret r: no_event_l (Ret r)
-  | Vis f k: (∀ t, no_event_l (k t)) → no_event_l (Vis (Sum.inr f) k)
+@[simp] theorem Fitree.translate_ret:
+  Fitree.translate f (Fitree.ret r) = Fitree.ret r := rfl
+@[simp] theorem Fitree.translate_vis:
+    Fitree.translate f (Vis e k) = Vis (f _ e) (fun r => translate f (k r)) :=
+  rfl
 
--- TODO: Tactic to automate the proof of no_event_l
+@[simp_itree]
+def Fitree.case (h₁: E ~> G) (h₂: F ~> G): E +' F ~> G :=
+  fun R ef => match ef with
+  | Sum.inl e => h₁ R e
+  | Sum.inr f => h₂ R f
+
+@[simp] theorem Fitree.case_left:
+  Fitree.case h₁ h₂ _ (Sum.inl e) = h₁ _ e := rfl
+@[simp] theorem Fitree.case_right:
+  Fitree.case h₁ h₂ _ (Sum.inr e) = h₂ _ e := rfl
+
+/-
+### Monadic interpretation
+-/
+
+@[simp_itree]
+def Fitree.interp {M} [Monad M] {E} (h: E ~> M) {R}: Fitree E R → M R
+  | .Ret r => pure r
+  | .Vis e k => Bind.bind (h _ e) (fun t => interp h (k t))
+
+@[simp_itree]
+def Fitree.interp' {E F} (h: E ~> Fitree Void1) {R} (t: Fitree (E +' F) R):
+    Fitree F R :=
+  interp (Fitree.case
+    (fun _ e => (h _ e).translate $ fun _ e => nomatch e)
+    (fun _ e => Fitree.trigger e)) t
+
+-- Interp `F` by lifting into a monad transformer (this is used when
+-- interpreting `E +' F` into the monad)
+def Fitree.liftHandler {F M} [MonadLiftT (Fitree F) M]: F ~> M := fun R e =>
+  monadLift (Fitree.trigger e: Fitree F R)
+
+-- Interpretation into various predefined monads. These are predefined so that
+-- rewriting theorems that expose the monad structure can be provided.
+
+@[simp_itree]
+def Fitree.interpState {M S} [Monad M] {E} (h: E ~> StateT S M):
+    forall {R}, Fitree E R → StateT S M R :=
+  interp h
+
+@[simp_itree]
+def Fitree.interpWriter {M} [Monad M] {E} (h: E ~> WriterT M):
+    forall {R}, Fitree E R → WriterT M R :=
+  interp h
+
+@[simp_itree]
+def Fitree.interpOption {M} [Monad M] {E} (h: E ~> OptionT M):
+    forall {R}, Fitree E R → OptionT M R :=
+  interp h
+
+@[simp_itree]
+def Fitree.interpExcept {M ε} [Monad M] {E} (h: E ~> ExceptT ε M) {R}:
+    Fitree E R → ExceptT ε M R :=
+  interp h
+
+/-
+### Combinator identities
+
+The following theorems act as the main interface for computation on ITrees. We
+don't unfold definitions because Lean 4 doesn't yet have the match-unfolding
+behavior of Coq's `simpl` tactic, and runs into performance issues as unfolded
+terms grow larger. Instead, we aggressively rewrite the following simplifying
+equalities.
+-/
+
+@[simp] theorem Fitree.bind_ret:
+  Fitree.bind (Fitree.ret r) k = k r := rfl
+
+@[simp] theorem Fitree.bind_ret':
+    Fitree.bind t (fun r => Fitree.ret r) = t := by
+  induction t with
+  | Ret _ => rfl
+  | Vis _ _ ih => simp [bind, ih]
+
+@[simp] theorem Fitree.bind_bind:
+    Fitree.bind (Fitree.bind t k) k' =
+    Fitree.bind t (fun x => Fitree.bind (k x) k') := by
+  induction t with
+  | Ret _ => rfl
+  | Vis _ _ ih => simp [bind, ih]
+
+@[simp] theorem Fitree.pure_is_ret:
+  @Pure.pure (Fitree E) _ _ r = Fitree.ret r := rfl
+
+@[simp] theorem Fitree.bind_is_bind:
+  @Bind.bind (Fitree E) _ _ _  t k = Fitree.bind t k := rfl
+
+@[simp] theorem Fitree.StateT_bind_is_bind (k: T → S → Fitree E (R × S)):
+  StateT.bind (m := Fitree E) t k =
+    fun s => Fitree.bind (t s) (fun (x,s) => k x s) := rfl
+
+@[simp] theorem Fitree.WriterT_bind_is_bind (k: T → Fitree E (R × String)):
+  WriterT.bind (m := Fitree E) t k =
+    Fitree.bind t (WriterT.bindCont k) := rfl
+
+@[simp] theorem Fitree.OptionT_bind_is_bind (k: T → Fitree E (Option R)):
+  OptionT.bind (m := Fitree E) t k =
+    Fitree.bind t (fun
+      | some x => k x
+      | none => Fitree.ret none) := rfl
+
+@[simp] theorem Fitree.ExceptT_bind_is_bind (k: T → Fitree E (Except ε R)):
+  ExceptT.bind (m := Fitree E) t k = Fitree.bind t (ExceptT.bindCont k) := rfl
+
+@[simp] theorem Fitree.liftHandler_StateT_is_StateT_lift:
+  @Fitree.liftHandler F (StateT S (Fitree F)) _ _ e =
+  fun s => Fitree.bind (Fitree.trigger e) (fun x => Fitree.ret (x, s)) := rfl
+
+@[simp] theorem Fitree.liftHandler_WriterT_is_WriterT_lift:
+  @Fitree.liftHandler F (WriterT (Fitree F)) _ _ e =
+  Fitree.bind (Fitree.trigger e) (fun x => Fitree.ret (x, "")) := rfl
+
+@[simp] theorem Fitree.liftHandler_OptionT_is_OptionT_lift:
+  @Fitree.liftHandler F (OptionT (Fitree F)) _ _ e =
+  Fitree.bind (Fitree.trigger e) (fun x => Fitree.ret (some x)) := rfl
+
+@[simp] theorem Fitree.liftHandler_ExceptT_is_ExceptT_lift:
+  @Fitree.liftHandler F (ExceptT ε (Fitree F)) _ _ e =
+  Fitree.bind (Fitree.trigger e) (fun x => Fitree.ret (Except.ok x)) := rfl
+
+@[simp] theorem Member.injectId:
+  @Member.inject E E MemberId _ e = e := rfl
+
+@[simp] theorem Member.injectSumL [Member E F]:
+  @Member.inject E (F +' G) MemberSumL _ e = Sum.inl (Member.inject _ e) := rfl
+
+@[simp] theorem Member.injectSumR [Member E G]:
+  @Member.inject E (F +' G) MemberSumR _ e = Sum.inr (Member.inject _ e) := rfl
+
+@[simp] theorem Member.injectSum_inl [Member E G] [Member F H]:
+  @Member.inject (E +' F) (G +' H) MemberSum _ (Sum.inl e) =
+    Sum.inl (Member.inject _ e) := rfl
+
+@[simp] theorem Member.injectSum_inr [Member E G] [Member F H]:
+  @Member.inject (E +' F) (G +' H) MemberSum _ (Sum.inr e) =
+    Sum.inr (Member.inject _ e) := rfl
+
+-- Interpretatin identities
 
 
-/- Rewriting tactic simp_itree -/
+@[simp] theorem Fitree.interp_ret:
+  Fitree.interp h (Fitree.ret r) = Fitree.ret r := rfl
+
+@[simp] theorem Fitree.interp_Vis:
+  Fitree.interp h (Fitree.Vis e k) =
+  Fitree.bind (h _ e) (fun x => Fitree.interp h (k x)) := rfl
+
+@[simp] theorem Fitree.interp'_ret:
+  @Fitree.interp' E F h _ (Fitree.ret r) = Fitree.ret r := rfl
+
+@[simp] theorem Fitree.interp'_Vis_left:
+  @Fitree.interp' E F h _ (Fitree.Vis (Sum.inl e) k) =
+  Fitree.bind (Fitree.translate (fun _ e => nomatch e) (h _ e))
+              (fun x => Fitree.interp' h (k x)) := rfl
+
+@[simp] theorem Fitree.interp'_Vis_right:
+  @Fitree.interp' E F h _ (Fitree.Vis (Sum.inr e) k) =
+  Fitree.bind (Fitree.trigger e)
+              (fun x => Fitree.interp' h (k x)) := rfl
+
+@[simp] theorem Fitree.interpState_ret:
+  Fitree.interpState h (Fitree.ret r) = (fun s => Fitree.ret (r, s)) := rfl
+
+@[simp] theorem Fitree.interpState_Vis {M S} [Monad M] (h: E ~> StateT S M):
+  Fitree.interpState h (Fitree.Vis e k) =
+  StateT.bind (h _ e) (fun x => Fitree.interpState h (k x)) := rfl
+
+@[simp] theorem Fitree.interpWriter_ret:
+  Fitree.interpWriter h (Fitree.ret r) = Fitree.ret (r, "") := rfl
+
+@[simp] theorem Fitree.interpWriter_Vis {M} [Monad M] (h: E ~> WriterT M):
+  Fitree.interpWriter h (Fitree.Vis e k) =
+  WriterT.bind (h _ e) (fun x => Fitree.interpWriter h (k x)) := rfl
+
+@[simp] theorem Fitree.interpOption_ret:
+  Fitree.interpOption h (Fitree.ret r) = Fitree.ret (some r) := rfl
+
+@[simp] theorem Fitree.interpOption_Vis {M} [Monad M] (h: E ~> OptionT M):
+  Fitree.interpOption h (Fitree.Vis e k) =
+  OptionT.bind (h _ e) (fun x => Fitree.interpOption h (k x)) := rfl
+
+@[simp] theorem Fitree.interpExcept_ret:
+  Fitree.interpExcept h (Fitree.ret r) = Fitree.ret (.ok r) := rfl
+
+@[simp] theorem Fitree.interpExcept_Vis {M ε} [Monad M] (h: E ~> ExceptT ε M):
+  Fitree.interpExcept h (Fitree.Vis e k) =
+  ExceptT.bind (h _ e) (fun x => Fitree.interpExcept h (k x)) := rfl
+
+-- We don't assume [LawfulMonad M] so we can't simplify the continuation. But
+-- when it's an ITree the other simp lemmas will do it anyway.
+@[simp] theorem Fitree.interp_trigger [Member E F] [Monad M] (e: E T):
+  Fitree.interp (M := M) (E := F) h (Fitree.trigger e) =
+  Bind.bind (h _ (Member.inject _ e)) (fun x => pure x) := rfl
+
+@[simp] theorem Fitree.interp'_trigger_left (e: E R):
+  @Fitree.interp' E F h _ (@Fitree.trigger (E +' F) _ _ MemberId (Sum.inl e)) =
+  Fitree.bind
+    (Fitree.translate (fun _ e => nomatch e) (h _ (Member.inject _ e)))
+    (fun x => pure x) := rfl
+
+@[simp] theorem Fitree.interp'_trigger_right [Member G F]:
+  @Fitree.interp' E F h _ (@Fitree.trigger (E +' G) (E +' F) _ _ (Sum.inr e)) =
+  Fitree.trigger e := rfl
+
+-- The following theorems are only applied manually
+
+theorem Fitree.interp_bind:
+    Fitree.interp h (Fitree.bind t k) =
+    Fitree.bind (Fitree.interp h t) (fun x => Fitree.interp h (k x)) := by
+  induction t with
+  | Ret _ => rfl
+  | Vis _ _ ih => simp [bind, ih]
+
+theorem Fitree.interp'_bind:
+    Fitree.interp' h (Fitree.bind t k) =
+    Fitree.bind (Fitree.interp' h t) (fun x => Fitree.interp' h (k x)) := by
+  simp [interp', interp_bind]
+
+-- Specialized interp_bind lemmas that unfold the monadic structure and expose
+-- the Fitree.bind directly rather than the monadic Bind.bind
+
+theorem Fitree.interpState_bind (h: E ~> StateT S (Fitree F)) (t: Fitree E R):
+    Fitree.interpState h (Fitree.bind t k) s =
+    Fitree.bind (Fitree.interpState h t s)
+      (fun (x,s') => Fitree.interpState h (k x) s') := by
+  revert s
+  induction t with
+  | Ret _ => intros s; rfl
+  | Vis _ _ ih =>
+    simp [interpState] at *
+    simp [interp, Bind.bind, StateT.bind]
+    simp [ih]
+
+example {F R}: WriterT (Fitree F) R = Fitree F (R × String) := by
+  simp [WriterT]
+
+theorem Fitree.interpWriter_bind (h: E ~> WriterT (Fitree F))
+  (t: Fitree E T) (k: T → Fitree E R):
+    Fitree.interpWriter h (Fitree.bind t k) =
+    Fitree.bind (Fitree.interpWriter h t) fun (x,s₁) =>
+      Fitree.bind (Fitree.interpWriter h (k x)) fun (y,s₂) =>
+        Fitree.ret (y,s₁++s₂) := by
+  induction t with
+  | Ret _ =>
+      simp [bind, interpWriter]
+      have h₁: forall x, "" ++ x = x := by
+        simp [HAppend.hAppend, Append.append, String.append]
+        simp [List.nil_append]
+      simp [h₁]
+      have h₂: forall (α β: Type) (x: α × β), (x.fst, x.snd) = x := by simp
+      simp [h₂]
+  | Vis _ _ ih =>
+      simp [interpWriter] at *
+      simp [interp, Bind.bind, WriterT.bindCont, WriterT.mk]
+      have h: forall (x y z: String), x ++ (y ++ z) = x ++ y ++ z := by
+        simp [HAppend.hAppend, Append.append, String.append]
+        simp [List.append_assoc]
+      simp [ih, h]
+
+theorem Fitree.interpOption_bind (h: E ~> OptionT (Fitree F))
+  (t: Fitree E T) (k: T → Fitree E R):
+    Fitree.interpOption h (Fitree.bind t k) =
+    Fitree.bind (Fitree.interpOption h t) fun x? =>
+      match x? with
+      | some x => Fitree.interpOption h (k x)
+      | none => Fitree.ret none := by
+  induction t with
+  | Ret _ => rfl
+  | Vis _ _ ih =>
+      simp [interpOption] at *
+      simp [interp, bind, Bind.bind, OptionT.bind, OptionT.mk]
+      -- I can't get a bind (match) → match (bind) theorem to rewrite, so...
+      have fequal2 α β (f g: α → β) x y: f = g → x = y → f x = g y :=
+        fun h₁ h₂ => by simp [h₁, h₂]
+      apply fequal2; rfl; funext x
+      cases x <;> simp [ih]
+
+theorem Fitree.interpExcept_bind (h: E ~> ExceptT ε (Fitree F))
+  (t: Fitree E T) (k: T → Fitree E R):
+    Fitree.interpExcept h (Fitree.bind t k) =
+    Fitree.bind (Fitree.interpExcept h t) fun x? =>
+      match x? with
+      | .error ε => Fitree.ret (.error ε)
+      | .ok x => Fitree.interpExcept h (k x) := by
+  induction t with
+  | Ret _ => rfl
+  | Vis _ _ ih =>
+      simp [interpExcept] at *
+      simp [interp, bind, Bind.bind]
+      simp [ExceptT.bind, ExceptT.mk, ExceptT.bindCont]
+      -- See above
+      have fequal2 α β (f g: α → β) x y: f = g → x = y → f x = g y :=
+        fun h₁ h₂ => by simp [h₁, h₂]
+      apply fequal2; rfl; funext x
+      cases x <;> simp [ih]
+
+-- This theorem has the drawback of hiding the continuation of `bind` into the
+-- `Vis` node, which blocks other theorems like `Fitree.bind_bind`.
+theorem Fitree.bind_trigger [Member E F] (e: E T) (k: T → Fitree F R):
+  Fitree.bind (Fitree.trigger e) k = Fitree.Vis (Member.inject _ e) k := rfl
+
+/-
+### Other properties
+-/
+
+inductive Fitree.noEventL {E F R}: Fitree (E +' F) R → Prop :=
+  | Ret r: noEventL (Ret r)
+  | Vis f k: (∀ t, noEventL (k t)) → noEventL (Vis (Sum.inr f) k)
+
+
+/-
+### Automation tools
+-/
+
+/- Rewriting tactics `simp_itree` and `dsimp_itree` -/
 
 open Lean Elab.Tactic Parser.Tactic
 
@@ -188,6 +444,7 @@ elab "simp_itree" : tactic => do
   let trlemmas: Syntax.TSepArray `Lean.Parser.Tactic.simpStar "," :=
     ⟨lemmas.reverse⟩
   evalTactic $ ← `(tactic|simp [$trlemmas,*,
+    Fitree.liftHandler,
     Member.inject,
     StateT.bind, StateT.pure, StateT.lift,
     OptionT.bind, OptionT.pure, OptionT.mk, OptionT.lift,
