MLIR/Semantics/Semantics.lean
@@ -19,15 +19,15 @@ abbrev TypedArgs (δ: Dialect α σ ε) := List ((τ: MLIRType δ) × MLIRType.e
 
 -- | TODO: throw error if we don't have enough names
 def denoteTypedArgs (args: TypedArgs Δ) (names: List SSAVal): Fitree (UBE +' SSAEnvE Δ) PUnit :=
- match args with 
+ match args with
  | [] => return ()
  | ⟨τ, val⟩::args =>
-    match names with 
+    match names with
     | [] => return ()
-    | name :: names => do 
+    | name :: names => do
         Fitree.trigger (SSAEnvE.Set τ name val)
         return ()
-    
+
 
 -- TODO: Consider changing BlockResult.Branch.args into
 --       a TypedArgs (?)
@@ -37,7 +37,7 @@ inductive BlockResult {α σ ε} (δ: Dialect α σ ε)
 | Next (val: (τ: MLIRType δ) × τ.eval)
 
 def BlockResult.toTypedArgs {δ: Dialect α σ ε} (blockResult: BlockResult δ) :=
-  match blockResult with 
+  match blockResult with
   | .Branch bb args => []
   | .Ret rets => rets
   | .Next val => []
@@ -112,9 +112,9 @@ def denoteOp (op: Op Δ):
       -- Use the dialect-provided semantics, and substitute regions
       match S.semantics_op iop with
       | some t =>
-          interp (fun _ e =>
+          Fitree.interp (fun _ e =>
             match e with
-            | Sum.inl (RegionE.RunRegion i xs) => 
+            | Sum.inl (RegionE.RunRegion i xs) =>
                  regions.get! i xs
             | Sum.inr <| Sum.inl ube => Fitree.trigger ube
             | Sum.inr <| Sum.inr se => Fitree.trigger se
@@ -143,26 +143,26 @@ def denoteBBStmt (bbstmt: BasicBlockStmt Δ):
 
 def denoteBBStmts (stmts: List (BasicBlockStmt Δ))
   : Fitree (UBE +' SSAEnvE Δ +' S.E) (BlockResult Δ) :=
- match stmts with 
+ match stmts with
  | [] => return BlockResult.Next ⟨.unit, ()⟩
  | [stmt] => denoteBBStmt stmt
- | stmt::stmts => do 
+ | stmt::stmts => do
       let _ ← denoteBBStmt stmt
       denoteBBStmts stmts
 
 def denoteBB (bb: BasicBlock Δ) (args: TypedArgs Δ := []):
     Fitree (UBE +' SSAEnvE Δ +' S.E) (BlockResult Δ) := do
-  match bb with 
-  | BasicBlock.mk name formalArgsAndTypes stmts => 
+  match bb with
+  | BasicBlock.mk name formalArgsAndTypes stmts =>
      -- TODO: check that types in [TypedArgs] is equal to types at [bb.args]
      -- TODO: Any checks on the BlockResults of intermediate ops?
      let formalArgs : List SSAVal:= formalArgsAndTypes.map Prod.fst
-     Fitree.inject (denoteTypedArgs args formalArgs)
+     Fitree.translate Member.inject (denoteTypedArgs args formalArgs)
      denoteBBStmts stmts
 
 def denoteRegions (rs: List (Region Δ)):
-    List (TypedArgs Δ → Fitree (UBE +' SSAEnvE Δ +' S.E) (BlockResult Δ)) := 
- match rs with 
+    List (TypedArgs Δ → Fitree (UBE +' SSAEnvE Δ +' S.E) (BlockResult Δ)) :=
+ match rs with
  | [] => []
  | r :: rs => (denoteRegion r) :: denoteRegions rs
 
@@ -190,7 +190,7 @@ instance
   semantics_op op :=
     (S₁.semantics_op op).map (.translate Member.inject) <|>
     (S₂.semantics_op op).map (.translate Member.inject)
-  handle := Fitree.case_ S₁.handle S₂.handle
+  handle := Fitree.case S₁.handle S₂.handle
 
 
 
@@ -221,24 +221,24 @@ def run! {Δ: Dialect α' σ' ε'} [S: Semantics Δ] {R}
     (t: Fitree (UBE +' SSAEnvE Δ +' S.E) R) (env: SSAEnv Δ):
     R × SSAEnv Δ :=
   let t := interp_ub! t
-  let t := interp_ssa t env
-  let t := interp S.handle t
+  let t := interpSSA' t env
+  let t := t.interp S.handle
   t.run
 
 def run {Δ: Dialect α' σ' ε'} [S: Semantics Δ] {R}
     (t: Fitree (UBE +' SSAEnvE Δ +' S.E) R) (env: SSAEnv Δ):
     Option R × SSAEnv Δ :=
   let t := interp_ub t
-  let t := interp_ssa t env
-  let t := interp S.handle t
+  let t := interpSSA' t env
+  let t := t.interp S.handle
   t.run
 
 def runLogged {Gα Gσ Gε} {Gδ: Dialect Gα Gσ Gε} [S: Semantics Gδ]
     {R} (t: Fitree (UBE +' SSAEnvE Gδ +' S.E) R) (env: SSAEnv Gδ):
     (R × String) × SSAEnv Gδ :=
   let t := interp_ub! t
-  let t := (interp_ssa_logged t).run env
-  let t := interp S.handle t
+  let t := (interpSSALogged' t).run env
+  let t := t.interp S.handle
   t.run
 
 
